verified_printer/Doc.v
@@ -1,0 +1,14 @@
+Require Import String.
+Open Scope list_scope.
+Require Import ZArith Int.
+Require Import Coq.Lists.List.
+Require Import Format.
+
+Inductive Doc : Type :=
+  | Text (s: string)
+  | Indent (t: nat) (d: Doc)
+  | Beside (d: Doc) (d: Doc)
+  | Above (d: Doc) (d: Doc)
+  | Choice (d: Doc) (d: Doc)
+  | Fill (d: Doc) (d: Doc) (s: nat).
+
