verified_printer/FormatTrivial.v
@@ -1,0 +1,46 @@
+Require Import Format.
+Require Import Doc.
+
+Open Scope list_scope.
+Require Import ZArith Int.
+Require Import Coq.Lists.List.
+Require Import String.
+
+Definition cross_general (width: nat) (op: t -> t -> t) (fl1: list t) (fl2: list t) :=
+  List.filter 
+    (fun f => total_width f <=? width)
+    (List.concat (map (fun b => map (fun a => op a b) fl1) fl2)).
+
+Definition blank_line := (line "")::nil.
+
+(* Construct document from 'string' using 'above' rule *)
+Definition constructDoc (s: string) := (of_string s)::nil.
+
+Definition indentDoc (width: nat) (shift: nat) (fs: list t) :=
+  cross_general width (fun _ b => indent' shift b) (empty::nil) fs.
+
+(* Use 'beside' rule for 2 documents. New document ~ n x m *)
+Definition besideDoc (width: nat) (fs1: list t) (fs2: list t) := 
+  cross_general width add_beside fs1 fs2.
+
+(* Use 'above' rule for 2 documents. New document ~ n x m *)
+Definition aboveDoc (width: nat) (fs1: list t) (fs2: list t) := 
+   cross_general width add_above fs1 fs2.
+
+(* 'Fill' rule *)
+Definition fillDoc (width: nat) (fs1: list t) (fs2: list t) (shift: nat) :=
+   cross_general width (fun fs f => add_fill fs f shift) fs1 fs2.
+
+(* Choice operation *)
+Definition choiceDoc (fs1: list t) (fs2: list t) := 
+    fs1 ++ fs2.
+
+Fixpoint evaluatorTrivial (width: nat) (doc: Doc): list t:=
+  match doc with
+  | Text s     => constructDoc s
+  | Indent n d => indentDoc width n (evaluatorTrivial width d)
+  | Beside a b => besideDoc width (evaluatorTrivial width a) (evaluatorTrivial width b)
+  | Above a b  => aboveDoc width (evaluatorTrivial width a) (evaluatorTrivial width b)
+  | Choice a b => choiceDoc (evaluatorTrivial width a) (evaluatorTrivial width b)
+  | Fill a b n => fillDoc width (evaluatorTrivial width a) (evaluatorTrivial width b) n
+  end.
